src/PermTypeProofs.v
@@ -49,25 +49,25 @@ Qed.
 Instance lens_config : Lens Si config := lens_config'.
 
 Lemma TrueI (A : Type) P (xi : A) :
-  P * xi : trueP Si Ss @ tt ⊑ P.
+  P * xi : trueP Si Ss ▷ tt ⊑ P.
 Proof.
   simpl. rewrite sep_conj_Perms_commut. rewrite sep_conj_Perms_bottom_identity. reflexivity.
 Qed.
 
 Lemma SumI1 (A1 A2 B1 B2 : Type) (xi : A1) (xs : B1) (T1 : PermType Si Ss A1 B1) (T2 : PermType Si Ss A2 B2) :
-  xi : T1 @ xs ⊑ inl xi : T1 +T+ T2 @ inl xs.
+  xi : T1 ▷ xs ⊑ inl xi : T1 +T+ T2 ▷ inl xs.
 Proof. reflexivity. Qed.
 
 Lemma SumI2 (A1 A2 B1 B2 : Type) (xi : A2) (xs : B2) (T1 : PermType Si Ss A1 B1) (T2 : PermType Si Ss A2 B2) :
-  xi : T2 @ xs ⊑ inr xi : T1 +T+ T2 @ inr xs.
+  xi : T2 ▷ xs ⊑ inr xi : T1 +T+ T2 ▷ inr xs.
 Proof. reflexivity. Qed.
 
 Lemma SumE (A1 A2 B1 B2 R1 R2 : Type)
       (xi : A1 + A2) (xs : B1 + B2) ti1 ti2 ts1 ts2
       (T1 : PermType Si Ss A1 B1) (T2 : PermType Si Ss A2 B2) (P : Perms) (U : PermType Si Ss (A1 + A2) (B1 + B2)) :
-  (forall yi ys, P * yi : T1 @ ys ⊢ ti1 ▷ ts1 ::: U) ->
-  (forall yi ys, P * yi : T2 @ ys ⊢ ti2 ▷ ts2 ::: U) ->
-  P * xi : T1 +T+ T2 @ xs ⊢ either (fun _ => ti1) (fun _ => ti2) xi ▷ either (fun _ => ts1) (fun _ => ts2) xs ::: U.
+  (forall yi ys, P * yi : T1 ▷ ys ⊢ ti1 ⤳ ts1 ::: U) ->
+  (forall yi ys, P * yi : T2 ▷ ys ⊢ ti2 ⤳ ts2 ::: U) ->
+  P * xi : T1 +T+ T2 ▷ xs ⊢ either (fun _ => ti1) (fun _ => ti2) xi ⤳ either (fun _ => ts1) (fun _ => ts2) xs ::: U.
 Proof.
   intros. simpl.
   destruct xi, xs; auto;
@@ -75,64 +75,62 @@ Proof.
 Qed.
 
 Lemma ProdI (A1 A2 B1 B2 : Type) xi yi xs ys (T1 : PermType Si Ss A1 B1) (T2 : PermType Si Ss A2 B2) :
-  xi : T1 @ xs * yi : T2 @ ys ⊑ (xi, yi) : T1 *T* T2 @ (xs, ys).
+  xi : T1 ▷ xs * yi : T2 ▷ ys ⊑ (xi, yi) : T1 *T* T2 ▷ (xs, ys).
 Proof. reflexivity. Qed.
 
 Lemma ProdE (A1 A2 B1 B2 : Type) xi xs (T1 : PermType Si Ss A1 B1) (T2 : PermType Si Ss A2 B2) :
-  xi : T1 *T* T2 @ xs ⊑ fst xi : T1 @ fst xs * snd xi : T2 @ snd xs.
+  xi : T1 *T* T2 ▷ xs ⊑ fst xi : T1 ▷ fst xs * snd xi : T2 ▷ snd xs.
 Proof. reflexivity. Qed.
 
 Lemma StarI (A B1 B2 : Type) xi xs ys (T1 : PermType Si Ss A B1) (T2 : PermType Si Ss A B2) :
-  xi : T1 @ xs * xi : T2 @ ys ⊑ xi : (starPT _ _ T1 T2) @ (xs, ys).
+  xi : T1 ▷ xs * xi : T2 ▷ ys ⊑ xi : (starPT _ _ T1 T2) ▷ (xs, ys).
 Proof. reflexivity. Qed.
 
 Lemma StarE (A B1 B2 : Type) xi xs (T1 : PermType Si Ss A B1) (T2 : PermType Si Ss A B2) :
-  xi : (starPT _ _ T1 T2) @ xs ⊑ xi : T1 @ fst xs * xi : T2 @ snd xs.
+  xi : (starPT _ _ T1 T2) ▷ xs ⊑ xi : T1 ▷ fst xs * xi : T2 ▷ snd xs.
 Proof. reflexivity. Qed.
 
 Lemma OrI1 (A B1 B2 : Type) xi xs (T1 : PermType Si Ss A B1) (T2 : PermType Si Ss A B2) :
-  xi : T1 @ xs ⊑ xi : (or _ _ T1 T2) @ inl xs.
+  xi : T1 ▷ xs ⊑ xi : (or _ _ T1 T2) ▷ inl xs.
 Proof. reflexivity. Qed.
 
 Lemma OrI2 (A B1 B2 : Type) xi xs (T1 : PermType Si Ss A B1) (T2 : PermType Si Ss A B2) :
-  xi : T2 @ xs ⊑ xi : (or _ _ T1 T2) @ inr xs.
+  xi : T2 ▷ xs ⊑ xi : (or _ _ T1 T2) ▷ inr xs.
 Proof. reflexivity. Qed.
 
 Lemma OrE (A B1 B2 R1 R2 : Type)
       (xi : A) (xs : B1 + B2) ti ts1 ts2
       (T1 : PermType Si Ss A B1) (T2 : PermType Si Ss A B2) (P : Perms) (U : PermType Si Ss A (B1 + B2)) :
-  (forall yi ys, P * yi : T1 @ ys ⊢ ti ▷ ts1 ::: U) ->
-  (forall yi ys, P * yi : T2 @ ys ⊢ ti ▷ ts2 ::: U) ->
-  P * xi : (or _ _ T1 T2) @ xs ⊢ ti ▷ either (fun _ => ts1) (fun _ => ts2) xs ::: U.
+  (forall yi ys, P * yi : T1 ▷ ys ⊢ ti ⤳ ts1 ::: U) ->
+  (forall yi ys, P * yi : T2 ▷ ys ⊢ ti ⤳ ts2 ::: U) ->
+  P * xi : (or _ _ T1 T2) ▷ xs ⊢ ti ⤳ either (fun _ => ts1) (fun _ => ts2) xs ::: U.
 Proof.
   intros. destruct xs; simpl; auto.
 Qed.
 
-Notation "'ex' ( x 'uhh' A ) T" := (existsPT _ _ (As:=A) (fun x => T)) (at level 70).
-
 Lemma ExI (A B C : Type) (xi : A) (xs : C) ys (F : forall (b : B), PermType Si Ss A C) :
-  xi : ex (z uhh B) (F z) @ existT _ ys xs ⊑ xi : F ys @ xs.
+  xi : ex (z oftype B) (F z) ▷ existT _ ys xs ⊑ xi : F ys ▷ xs.
 Proof. reflexivity. Qed.
 
 Lemma ExE (A B C : Type) (xi : A) (xs : sigT (fun b : B => C)) (F : forall (b : B), PermType Si Ss A C) :
-   xi : F (projT1 xs) @ (projT2 xs) ⊑ xi : ex (z uhh B) (F z) @ xs.
+   xi : F (projT1 xs) ▷ (projT2 xs) ⊑ xi : ex (z oftype B) (F z) ▷ xs.
 Proof. reflexivity. Qed.
 
 Lemma Frame (A B : Type) (P1 P2 : Perms) ti ts (T : PermType Si Ss A B) :
-  P1 ⊢ ti ▷ ts ::: T ->
-  (P1 * P2) ⊢ ti ▷ ts ::: (T ∅ P2).
+  P1 ⊢ ti ⤳ ts ::: T ->
+  (P1 * P2) ⊢ ti ⤳ ts ::: (T ∅ P2).
 Proof. apply typing_frame. Qed.
 
 Lemma PermsI (A B : Type) (P : Perms) xi xs (T : PermType Si Ss A B) :
-  xi : T @ xs * P ⊑ xi : T ∅ P @ xs.
+  xi : T ▷ xs * P ⊑ xi : T ∅ P ▷ xs.
 Proof. reflexivity. Qed.
 
 Lemma PermsE (A B : Type) (P : Perms) xi xs (T : PermType Si Ss A B) :
-  xi : T ∅ P @ xs ⊑ xi : T @ xs * P.
+  xi : T ∅ P ▷ xs ⊑ xi : T ▷ xs * P.
 Proof. reflexivity. Qed.
 
 Lemma Cast (A B : Type) (P : PermType Si Ss A B) xi yi xs ys :
-  xi : P @ ys ⊑ xi : eqp _ _ yi @ xs * yi : P @ ys.
+  xi : P ▷ ys ⊑ xi : eqp _ _ yi ▷ xs * yi : P ▷ ys.
 Proof.
   repeat intro. destruct H as (e & p' & Heq & Hp & Hlte).
   simpl in Heq. subst.
@@ -140,77 +138,77 @@ Proof.
 Qed.
 
 Lemma EqDup (A : Type) (xi yi : A) :
-  xi : eqp Si Ss yi @ tt * xi : eqp _ _ yi @ tt ⊑ xi : eqp _ _ yi @ tt.
+  xi : eqp Si Ss yi ▷ tt * xi : eqp _ _ yi ▷ tt ⊑ xi : eqp _ _ yi ▷ tt.
 Proof.
   repeat intro. simpl in *. subst. exists bottom_perm, bottom_perm.
   split; [| split]; auto. rewrite sep_conj_perm_bottom. apply bottom_perm_is_bottom.
 Qed.
 
 Lemma EqTrans (A : Type) (xi yi zi : A) :
-    xi : eqp Si Ss zi @ tt ⊑ xi : eqp _ _ yi @ tt * yi : eqp _ _ zi @ tt.
+    xi : eqp Si Ss zi ▷ tt ⊑ xi : eqp _ _ yi ▷ tt * yi : eqp _ _ zi ▷ tt.
 Proof.
   repeat intro. destruct H as (? & ? & ? & ? & ?). simpl in *; subst. reflexivity.
 Qed.
 
 Lemma EqCtx (A B : Type) (xi yi : A) (f : A -> B) :
-  f xi : eqp Si Ss (f yi) @ tt ⊑ xi : eqp _ _ yi @ tt.
+  f xi : eqp Si Ss (f yi) ▷ tt ⊑ xi : eqp _ _ yi ▷ tt.
 Proof.
   repeat intro. simpl in *. congruence.
 Qed.
 
 Lemma EqRefl A P (xi : A) :
-  P * xi : eqp Si Ss xi @ tt ⊑ P.
+  P * xi : eqp Si Ss xi ▷ tt ⊑ P.
 Proof.
   repeat intro.
   exists p, bottom_perm. split; [| split]; simpl; eauto. rewrite sep_conj_perm_bottom. reflexivity.
 Qed.
 
 Lemma EqSym (A : Type) (xi yi : A) :
-  yi : eqp Si Ss xi @ tt ⊑ xi : eqp _ _ yi @ tt.
+  yi : eqp Si Ss xi ▷ tt ⊑ xi : eqp _ _ yi ▷ tt.
 Proof.
   repeat intro; simpl in *; subst; reflexivity.
 Qed.
 
 Lemma Weak (A B : Type) P1 P2 (U1 U2 : PermType Si Ss A B) ts ti :
   P2 ⊑ P1 ->
-  (forall xi xs, xi : U1 @ xs ⊑ xi : U2 @ xs) ->
-  P2 ⊢ ts ▷ ti ::: U2 ->
-  P1 ⊢ ts ▷ ti ::: U1.
+  (forall xi xs, xi : U1 ▷ xs ⊑ xi : U2 ▷ xs) ->
+  P2 ⊢ ts ⤳ ti ::: U2 ->
+  P1 ⊢ ts ⤳ ti ::: U1.
 Proof.
   intros. eapply typing_lte; eauto.
 Qed.
 
 (* TODO name conflicts with ITree Ret *)
 Lemma Ret_ (A B : Type) xi xs (T : PermType Si Ss A B) :
-  xi : T @ xs ⊢ Ret xi ▷ Ret xs ::: T.
+  xi : T ▷ xs ⊢ Ret xi ⤳ Ret xs ::: T.
 Proof.
   repeat intro. pstep. constructor; auto.
 Qed.
 
 Lemma Bind (A B C D : Type) P ti ts fi fs (T : PermType Si Ss A B) (U : PermType Si Ss C D) :
-  P ⊢ ti ▷ ts ::: T ->
-  (forall xi xs, xi : T @ xs ⊢ fi xi ▷ fs xs ::: U) ->
-  P ⊢ ITree.bind ti fi ▷ ITree.bind ts fs ::: U.
+  P ⊢ ti ⤳ ts ::: T ->
+  (forall xi xs, xi : T ▷ xs ⊢ fi xi ⤳ fs xs ::: U) ->
+  P ⊢ ITree.bind ti fi ⤳ ITree.bind ts fs ::: U.
 Proof.
   intros. eapply typing_bind; eauto.
 Qed.
 
 Lemma GetNum xi yi :
-  xi : eqp Si Ss (VNum yi) @ tt ⊢ getNum xi ▷ Ret tt ::: eqp _ _ yi.
+  xi : eqp Si Ss (VNum yi) ▷ tt ⊢ getNum xi ⤳ Ret tt ::: eqp _ _ yi.
 Proof.
   repeat intro. simpl in *. subst. simpl. pstep. constructor; auto. reflexivity.
 Qed.
 
 Lemma Err (A B : Type) P (U : PermType Si Ss A B) t :
-  P ⊢ t ▷ throw tt ::: U.
+  P ⊢ t ⤳ throw tt ::: U.
 Proof.
   repeat intro. pstep. constructor.
 Qed.
 
 Lemma If (A B : Type) P ti1 ti2 ts1 ts2 (xi yi : bool) xs (U : PermType Si Ss A B) :
-  P ⊢ ti1 ▷ ts1 ::: U ->
-  P ⊢ ti2 ▷ ts2 ::: U ->
-  P * xi : eqp _ _ yi @ xs ⊢ if xi then ti1 else ti2 ▷ if yi then ts1 else ts2 ::: U.
+  P ⊢ ti1 ⤳ ts1 ::: U ->
+  P ⊢ ti2 ⤳ ts2 ::: U ->
+  P * xi : eqp _ _ yi ▷ xs ⊢ if xi then ti1 else ti2 ⤳ if yi then ts1 else ts2 ::: U.
 Proof.
   repeat intro. destruct H1 as (? & ? & ? & ? & ?); simpl in *; subst.
   destruct xi.
@@ -221,8 +219,8 @@ Proof.
 Qed.
 
 Lemma Iter (A B C D : Type) (T : PermType Si Ss C D) xi xs fi fs (U : PermType Si Ss A B) :
-  (forall yi ys, yi : T @ ys ⊢ fi yi ▷ fs ys ::: T +T+ U) ->
-  xi : T @ xs ⊢ iter fi xi ▷ iter fs xs ::: U.
+  (forall yi ys, yi : T ▷ ys ⊢ fi yi ⤳ fs ys ::: T +T+ U) ->
+  xi : T ▷ xs ⊢ iter fi xi ⤳ iter fs xs ::: U.
 Proof.
   revert xi xs fi fs U. pcofix CIH. intros.
   do 2 rewritebisim @unfold_iter_ktree.
@@ -242,10 +240,10 @@ Definition ex1s (xs : sigT (fun _ : nat => unit)) : itree (sceE Ss) (sigT (fun _
   Ret (existT _ (Init.Nat.mul 5 (projT1 xs)) tt).
 
 Definition IsNat : VPermType Si Ss (sigT (fun _ : nat => unit)) :=
-  ex (n uhh nat) eqp Si Ss (VNum n).
+  ex (n oftype nat) eqp Si Ss (VNum n).
 
 Lemma ex1_typing xi xs :
-  xi : IsNat @ xs ⊢ ex1i xi ▷ ex1s xs ::: IsNat.
+  xi : IsNat ▷ xs ⊢ ex1i xi ⤳ ex1s xs ::: IsNat.
 Proof.
   (* ExE *)
   unfold IsNat. eapply Weak; [eapply ExE | reflexivity |].
@@ -263,7 +261,7 @@ Proof.
 Qed.
 
 Lemma PtrI A xi yi xs ys rw o (T : VPermType Si Ss A) :
-  xi : ptr _ _ (rw, o, T) @ ys ⊑ xi : ptr _ _ (rw, o, eqp Si Ss yi) @ xs * yi : T @ ys.
+  xi : ptr _ _ (rw, o, T) ▷ ys ⊑ xi : ptr _ _ (rw, o, eqp Si Ss yi) ▷ xs * yi : T ▷ ys.
 Proof.
   destruct xi; simpl.
   - rewrite sep_conj_Perms_top_absorb. reflexivity.
@@ -278,8 +276,8 @@ Proof.
 Qed.
 
 Lemma ReadDup o xi yi xs:
-  xi : ptr _ _ (R, o, eqp Si Ss yi) @ xs * xi : ptr _ _ (R, o, eqp _ _ yi) @ xs ⊑
-  xi : ptr _ _ (R, o, eqp _ _ yi) @ xs.
+  xi : ptr _ _ (R, o, eqp Si Ss yi) ▷ xs * xi : ptr _ _ (R, o, eqp _ _ yi) ▷ xs ⊑
+  xi : ptr _ _ (R, o, eqp _ _ yi) ▷ xs.
 Proof.
   repeat intro. simpl in *. destruct xi; [contradiction |].
   destruct a as [b o']. unfold offset in *.
@@ -306,7 +304,7 @@ Qed.
 
 Lemma PtrOff A xi xs rw o1 o2 (T : VPermType Si Ss A) :
   o1 >= o2 ->
-  offset xi o2 : ptr _ _ (rw, o1 - o2, T) @ xs ⊑ xi : ptr _ _ (rw, o1, T) @ xs.
+  offset xi o2 : ptr _ _ (rw, o1 - o2, T) ▷ xs ⊑ xi : ptr _ _ (rw, o1, T) ▷ xs.
 Proof.
   destruct xi; [reflexivity | destruct a].
   intros. simpl. rewrite <- Nat.add_assoc. rewrite (Minus.le_plus_minus_r _ _ H).
@@ -314,8 +312,8 @@ Proof.
 Qed.
 
 Lemma PtrE A B C (P : Perms) rw o (T : VPermType Si Ss A) (xi yi : Value) xs ti ts (U : PermType Si Ss B C) :
-  (forall yi, P * xi : ptr _ _ (rw, o, eqp Si Ss yi) @ tt * yi : T @ xs ⊢ ti ▷ ts ::: U) ->
-  P * xi : ptr _ _ (rw, o, T) @ xs ⊢ ti ▷ ts ::: U.
+  (forall yi, P * xi : ptr _ _ (rw, o, eqp Si Ss yi) ▷ tt * yi : T ▷ xs ⊢ ti ⤳ ts ::: U) ->
+  P * xi : ptr _ _ (rw, o, T) ▷ xs ⊢ ti ⤳ ts ::: U.
 Proof.
   repeat intro. rename p into p''. destruct H0 as (p & p' & Hp & Hptr & Hlte).
   destruct xi; [contradiction | destruct a].
@@ -331,10 +329,10 @@ Proof.
 Qed.
 
 Lemma Load xi yi xs rw :
-  xi : ptr _ _ (rw, 0, eqp Si Ss yi) @ xs ⊢
-  load xi ▷
+  xi : ptr _ _ (rw, 0, eqp Si Ss yi) ▷ xs ⊢
+  load xi ⤳
   Ret tt :::
-  eqp _ _ yi ∅ xi : ptr _ _ (rw, 0, eqp _ _ yi) @ xs.
+  eqp _ _ yi ∅ xi : ptr _ _ (rw, 0, eqp _ _ yi) ▷ xs.
 Proof.
   repeat intro. pstep. unfold load. rewritebisim @bind_trigger.
   econstructor; eauto; try reflexivity.
@@ -357,10 +355,10 @@ Proof.
 Qed.
 
 Lemma Store A xi yi xs (P : VPermType Si Ss A) :
-  xi : ptr _ _ (W, 0, P) @ xs ⊢
-  store xi yi ▷
+  xi : ptr _ _ (W, 0, P) ▷ xs ⊢
+  store xi yi ⤳
   Ret tt :::
-  (trueP Si Ss) ∅ xi : ptr _ _ (W, 0, eqp _ _ yi) @ tt.
+  (trueP Si Ss) ∅ xi : ptr _ _ (W, 0, eqp _ _ yi) ▷ tt.
 Proof.
   repeat intro. pstep. unfold store. destruct xi as [| [b o]]; try contradiction.
   rewritebisim @bind_trigger.
@@ -411,23 +409,23 @@ Definition ex2s : itree (sceE Ss) unit :=
   Ret tt.
 
 Lemma ex2_typing A (xi yi : Value) xs (T : VPermType Si Ss A) :
-  xi : ptr _ _ (R, 0, T) @ xs * yi : ptr Si Ss (W, 0, trueP _ _) @ tt ⊢
-  ex2i xi yi ▷
+  xi : ptr _ _ (R, 0, T) ▷ xs * yi : ptr Si Ss (W, 0, trueP _ _) ▷ tt ⊢
+  ex2i xi yi ⤳
   ex2s :::
-  (trueP _ _) ∅ yi : ptr _ _ (W, 0, T) @ xs ∅ xi : ptr _ _ (R, 0, trueP _ _) @ tt.
+  (trueP _ _) ∅ yi : ptr _ _ (W, 0, T) ▷ xs ∅ xi : ptr _ _ (R, 0, trueP _ _) ▷ tt.
 Proof.
   rewrite sep_conj_Perms_commut.
   eapply PtrE; eauto.
   intros zi. eapply Bind.
   - apply Frame. rewrite sep_conj_Perms_commut. apply Frame. apply Load.
   - intros wi [].
-    eapply Weak with (P2 := yi : ptr _ _ (W, 0, trueP _ _) @ tt *
-                            wi : T @ xs *
-                            xi : ptr _ _ (R, 0, trueP _ _) @ tt)
+    eapply Weak with (P2 := yi : ptr _ _ (W, 0, trueP _ _) ▷ tt *
+                            wi : T ▷ xs *
+                            xi : ptr _ _ (R, 0, trueP _ _) ▷ tt)
                      (U2 := trueP _ _ ∅
-                            yi : ptr _ _ (W, 0, eqp _ _ wi) @ tt ∅
-                            wi : T @ xs ∅
-                            xi : ptr _ _ (R, 0, trueP _ _) @ tt).
+                            yi : ptr _ _ (W, 0, eqp _ _ wi) ▷ tt ∅
+                            wi : T ▷ xs ∅
+                            xi : ptr _ _ (R, 0, trueP _ _) ▷ tt).
 
     + etransitivity.
       2: {
@@ -437,7 +435,7 @@ Proof.
         eapply sep_conj_Perms_monotone; [reflexivity |]. (* frame *)
         etransitivity; [| apply PermsI]. rewrite sep_conj_Perms_commut. reflexivity.
       }
-      rewrite (sep_conj_Perms_commut (zi : T @ xs) _).
+      rewrite (sep_conj_Perms_commut (zi : T ▷ xs) _).
       repeat rewrite <- sep_conj_Perms_assoc.
       apply sep_conj_Perms_monotone; [reflexivity |].
       rewrite sep_conj_Perms_commut.
@@ -462,10 +460,10 @@ Proof.
 Qed.
 
 Lemma IsNull1 A xi xs rw o (P : VPermType Si Ss A) :
-  xi : ptr _ _ (rw, o, P) @ xs ⊢
-  isNull xi ▷
+  xi : ptr _ _ (rw, o, P) ▷ xs ⊢
+  isNull xi ⤳
   Ret tt :::
-  eqp _ _ false ∅ xi : ptr _ _ (rw, o, P) @ xs.
+  eqp _ _ false ∅ xi : ptr _ _ (rw, o, P) ▷ xs.
 Proof.
   repeat intro. pstep. unfold isNull. destruct xi; [contradiction |].
   destruct a as [b o']. simpl. constructor; auto.
@@ -474,8 +472,8 @@ Proof.
 Qed.
 
 Lemma IsNull2 xi:
-  xi : eqp Si Ss (VNum 0) @ tt ⊢
-  isNull xi ▷
+  xi : eqp Si Ss (VNum 0) ▷ tt ⊢
+  isNull xi ⤳
   Ret tt :::
   eqp _ _ true.
 Proof.
@@ -483,13 +481,13 @@ Proof.
 Qed.
 
 Lemma ArrPtr A xi xs rw o (P : VPermType Si Ss A) :
-  xi : ptr _ _ (rw, o, P) @ Vector.hd xs ⊑ xi : arr (rw, o, 1, P) @ xs.
+  xi : ptr _ _ (rw, o, P) ▷ Vector.hd xs ⊑ xi : arr (rw, o, 1, P) ▷ xs.
 Proof.
   simpl. rewrite sep_conj_Perms_commut. rewrite sep_conj_Perms_bottom_identity. reflexivity.
 Qed.
 
 Lemma PtrArr A xi xs rw o (P : VPermType Si Ss A) :
-  xi : arr (rw, o, 1, P) @ vsingle xs ⊑ xi : ptr _ _ (rw, o, P) @ xs.
+  xi : arr (rw, o, 1, P) ▷ vsingle xs ⊑ xi : ptr _ _ (rw, o, P) ▷ xs.
 Proof.
   simpl. rewrite sep_conj_Perms_commut. rewrite sep_conj_Perms_bottom_identity. reflexivity.
 Qed.
@@ -559,8 +557,8 @@ Definition trySplit {A l1 R S} (v : Vector.t A l1) l2 (f : Vector.t A l2 -> Vect
 Defined.
 
 Lemma ArrCombine_eq A xi rw o l1 l2 (l:le l2 l1) xs1 xs2 (P : VPermType Si Ss A) :
-  eq_Perms (xi : arr (rw, o, l1, P) @ append_leq l1 l2 l xs1 xs2)
-           (xi : arr (rw, o, l2, P) @ xs1 * xi : arr (rw, o + l2, l1 - l2, P) @ xs2).
+  eq_Perms (xi : arr (rw, o, l1, P) ▷ append_leq l1 l2 l xs1 xs2)
+           (xi : arr (rw, o, l2, P) ▷ xs1 * xi : arr (rw, o + l2, l1 - l2, P) ▷ xs2).
 Proof.
   revert o l2 l xs1 xs2; induction l1; intros.
   - inversion l. subst. simpl. rewrite sep_conj_Perms_bottom_identity. reflexivity.
@@ -575,10 +573,10 @@ Qed.
 
 Lemma ArrSplit A R1 R2 P l1 l2 xi xs rw o (T : VPermType Si Ss A) U (ti : itree (sceE Si) R1) (fs : _ -> _ -> itree (sceE Ss) R2) :
   (forall xs1 xs2, P *
-              xi : arr (rw, o, l2, T) @ xs1 *
-              xi : arr (rw, o + l2, l1 - l2, T) @ xs2 ⊢
-              ti ▷ fs xs1 xs2 ::: U) ->
-  P * xi : arr (rw, o, l1, T) @ xs ⊢ ti ▷ trySplit xs l2 fs ::: U.
+              xi : arr (rw, o, l2, T) ▷ xs1 *
+              xi : arr (rw, o + l2, l1 - l2, T) ▷ xs2 ⊢
+              ti ⤳ fs xs1 xs2 ::: U) ->
+  P * xi : arr (rw, o, l1, T) ▷ xs ⊢ ti ⤳ trySplit xs l2 fs ::: U.
 Proof.
   intros. unfold trySplit. destruct (le_lt_dec l2 l1).
   - rewrite <- (split_leq_append_leq _ l1 xs l2 l).
@@ -601,8 +599,8 @@ Proof.
 Qed.
 
 Lemma ArrCombine A xi rw o l1 l2 xs1 xs2 (P : VPermType Si Ss A) :
-  xi : arr (rw, o, l1 + l2, P) @ Vector.append xs1 xs2 ⊑
-  xi : arr (rw, o, l1, P) @ xs1 * xi : arr (rw, o + l1, l2, P) @ xs2.
+  xi : arr (rw, o, l1 + l2, P) ▷ Vector.append xs1 xs2 ⊑
+  xi : arr (rw, o, l1, P) ▷ xs1 * xi : arr (rw, o + l1, l2, P) ▷ xs2.
 Proof.
   repeat intro. destruct H as (p1 & p2 & Hp1 & Hp2 & Hlte).
   revert Hp1 Hp2. revert o xi l2 xs2. revert Hlte. revert p p1 p2. induction l1; intros.
@@ -621,7 +619,7 @@ Qed.
 Lemma MuFold A G X `{FixedPoint G X} (F:PermType Si Ss A X -> PermType Si Ss A (G X))
       {prp:Proper (lte_PermType _ _ ==> lte_PermType _ _) F}
       xi xs :
-  xi : mu _ _ F @ foldFP xs ⊑ xi : F (mu _ _ F) @ xs.
+  xi : mu _ _ F ▷ foldFP xs ⊑ xi : F (mu _ _ F) ▷ xs.
 Proof.
   (* FIXME: why can't we just rewrite with mu_fixed_point here? *)
   eapply Proper_eq_Perms_lte_Perms; [ | reflexivity | ].
@@ -632,7 +630,7 @@ Qed.
 Lemma MuUnfold A G X `{FixedPoint G X} (F:PermType Si Ss A X -> PermType Si Ss A (G X))
       {prp:Proper (lte_PermType _ _ ==> lte_PermType _ _) F}
       xi xs :
-  xi : F (mu _ _ F) @ unfoldFP xs ⊑ xi : mu _ _ F @ xs.
+  xi : F (mu _ _ F) ▷ unfoldFP xs ⊑ xi : mu _ _ F ▷ xs.
 Proof.
   eapply Proper_eq_Perms_lte_Perms; [ reflexivity | | ].
   - apply Proper_eq_PermType_ptApp; [ apply mu_fixed_point | | ]; reflexivity.
